use `G` instead of `g` for Graph variable

LeanHoG/Invariant/HamiltonianPath/Basic.lean
@@ -5,16 +5,16 @@ namespace LeanHoG
 
 /-- A path is Hamiltonian if it contains every vertex of a graph `g`. -/
 @[simp]
-def Path.isHamiltonian {g : Graph} {u v : g.vertex} (p : Path g u v) : Prop :=
-  ∀ (w : g.vertex), w ∈ p.walk.vertices
+def Path.isHamiltonian {G : Graph} {u v : G.vertex} (p : Path G u v) : Prop :=
+  ∀ (w : G.vertex), w ∈ p.walk.vertices
 
-instance {g : Graph} {u v : g.vertex} {p : Path g u v} :
+instance {G : Graph} {u v : G.vertex} {p : Path G u v} :
   Decidable (p.isHamiltonian) := by
   simp
   infer_instance
 
-def Graph.isTraceable (g : Graph) : Prop :=
-  ∃ (u v : g.vertex) (p : Path g u v), p.isHamiltonian
+def Graph.isTraceable (G : Graph) : Prop :=
+  ∃ (u v : G.vertex) (p : Path G u v), p.isHamiltonian
 
 lemma Graph.no_path_not_traceable {G : Graph}
   {h : ¬ ∃ (u v : G.vertex) (p : Path G u v), p.isHamiltonian} :
@@ -26,20 +26,20 @@ lemma Graph.no_path_not_traceable {G : Graph}
 /-- The class representing a Hamiltonian path of a graph `g`
     going from vertex `u` to vertex `v`.
  -/
-class HamiltonianPath (g : Graph) where
-  u : g.vertex
-  v : g.vertex
-  path : Path g u v
+class HamiltonianPath (G : Graph) where
+  u : G.vertex
+  v : G.vertex
+  path : Path G u v
   isHamiltonian : path.isHamiltonian := by decide
 namespace HamiltonianPath
 
-instance {g : Graph} : Repr (HamiltonianPath g) where
+instance {G : Graph} : Repr (HamiltonianPath G) where
   reprPrec p n := reprPrec p.path n
 
-instance {g : Graph} : ToString (HamiltonianPath g) where
+instance {G : Graph} : ToString (HamiltonianPath G) where
   toString p := toString p.path
 
-@[simp] theorem path_of_cert {g : Graph} [hp : HamiltonianPath g] : g.isTraceable := by
+@[simp] theorem path_of_cert {G : Graph} [hp : HamiltonianPath G] : G.isTraceable := by
   let ⟨u, v, p, cond⟩ := hp
   simp [Graph.isTraceable]
   apply Exists.intro u
@@ -50,31 +50,31 @@ instance {g : Graph} : ToString (HamiltonianPath g) where
 instance {G : Graph} [HamiltonianPath G] : Decidable (G.isTraceable) :=
   .isTrue path_of_cert
 
-@[simp] def vertices {g : Graph} : HamiltonianPath g → List g.vertex :=
+@[simp] def vertices {G : Graph} : HamiltonianPath G → List G.vertex :=
   fun p => p.path.vertices
 
-@[simp] lemma vertices_all_distinct {g : Graph} {hp : HamiltonianPath g} :
+@[simp] lemma vertices_all_distinct {G : Graph} {hp : HamiltonianPath G} :
   hp.vertices.all_distinct := by
   simp
   exact hp.path.isPath
 
-@[simp] def vertexMultiset {g : Graph} : HamiltonianPath g → Multiset g.vertex :=
+@[simp] def vertexMultiset {G : Graph} : HamiltonianPath G → Multiset G.vertex :=
   fun p => p.path.vertexMultiset
 
-@[simp] lemma vertexMultiset_nodup {g : Graph} {p : HamiltonianPath g} :
+@[simp] lemma vertexMultiset_nodup {G : Graph} {p : HamiltonianPath G} :
   Multiset.Nodup p.vertexMultiset := by
   apply Iff.mp Multiset.coe_nodup
   apply Iff.mp List.all_distinct_iff_nodup
   apply p.path.isPath
 
-@[simp] def vertexFinset {g : Graph} : HamiltonianPath g → Finset g.vertex := fun p =>
+@[simp] def vertexFinset {G : Graph} : HamiltonianPath G → Finset G.vertex := fun p =>
   ⟨p.vertexMultiset, vertexMultiset_nodup⟩
 
 /-- The length of a Hamiltonian path is just the length of the underlying path.
     This is not the same as the length of the path, as that is the number of
     edges of the path.
 -/
-@[simp] def length {g : Graph} : HamiltonianPath g → Nat :=
+@[simp] def length {G : Graph} : HamiltonianPath G → Nat :=
   fun p => p.path.length
 
 lemma lt_count_eq_one {n : Nat} : ∀ (k : Nat), k < n → List.count k (List.range n) = 1 := by
@@ -92,44 +92,44 @@ example {α : Type} [DecidableEq α] (l : List α) (d : l.Nodup) : Finset.card (
   apply List.toFinset_card_of_nodup d
 
 /-- The number of vertices on a Hamiltonian path is the number of vertices in the graph. -/
-@[simp] lemma length_eq_num_vertices {g : Graph} {hp : HamiltonianPath g} :
-  hp.vertices.length = g.vertexSize := by
+@[simp] lemma length_eq_num_vertices {G : Graph} {hp : HamiltonianPath G} :
+  hp.vertices.length = G.vertexSize := by
   let l := hp.vertices
   let ad : l.all_distinct := by apply hp.path.isPath
   have nd : l.Nodup := by apply Iff.mp List.all_distinct_iff_nodup ad
   have equiv := List.Nodup.getEquivOfForallMemList l nd hp.isHamiltonian
   simp at equiv
-  have : List.length l = g.vertexSize := by
+  have : List.length l = G.vertexSize := by
     apply Iff.mp Fin.equiv_iff_eq
     exact Nonempty.intro equiv
   exact this
 
 end HamiltonianPath
 
-@[simp] def Cycle.isHamiltonian {g : Graph} {u : g.vertex} (c : Cycle g u) : Bool :=
-  ∀ (v : g.vertex), List.contains c.cycle.vertices v
+@[simp] def Cycle.isHamiltonian {G : Graph} {u : G.vertex} (c : Cycle G u) : Bool :=
+  ∀ (v : G.vertex), List.contains c.cycle.vertices v
 
-class HamiltonianCycle (g : Graph)  where
-  u : g.vertex
-  cycle : Cycle g u
+class HamiltonianCycle (G : Graph)  where
+  u : G.vertex
+  cycle : Cycle G u
   isHamiltonian : cycle.isHamiltonian = true
 
-instance {g : Graph} : Repr (HamiltonianCycle g) where
+instance {G : Graph} : Repr (HamiltonianCycle G) where
   reprPrec p n := reprPrec p.cycle n
 
-instance {g : Graph} : Repr (HamiltonianCycle g) where
+instance {G : Graph} : Repr (HamiltonianCycle G) where
   reprPrec p n := reprPrec p.2.cycle n
 
-@[simp] def Graph.isHamiltonian (g : Graph) : Prop :=
-  ∃ (u : g.vertex) (c : Cycle g u), c.isHamiltonian
+@[simp] def Graph.isHamiltonian (G : Graph) : Prop :=
+  ∃ (u : G.vertex) (c : Cycle G u), c.isHamiltonian
 
-@[simp] def Graph.isNonHamiltonian (g : Graph) : Prop := ¬ g.isHamiltonian
+@[simp] def Graph.isNonHamiltonian (G : Graph) : Prop := ¬ G.isHamiltonian
 
-@[simp] def Graph.isNonHamiltonian' {g : Graph} : Prop :=
-  ∀ (u : g.vertex) (c : Cycle g u), ¬c.isHamiltonian
+@[simp] def Graph.isNonHamiltonian' {G : Graph} : Prop :=
+  ∀ (u : G.vertex) (c : Cycle G u), ¬c.isHamiltonian
 
-theorem equivNonHamiltonianDefs (g : Graph) :
-  g.isNonHamiltonian ↔ g.isNonHamiltonian' :=
+theorem equivNonHamiltonianDefs (G : Graph) :
+  G.isNonHamiltonian ↔ G.isNonHamiltonian' :=
   by simp
 
 end LeanHoG
